src/BinEncoders/Env/Examples/ByteAlignedExample.v
@@ -30,27 +30,12 @@ Definition Simple_Format_Spec
 Definition Simply_OK (p : simple_record) :=
   ((|snd p|) < pow2 8)%nat.
 
-Lemma zeta_to_fst {A B C}
-  : forall (ab : A * B) (k : A -> B -> C),
-    (let (a, b) := ab in (k a b)) =
-    k (fst ab) (snd ab).
-Proof.
-  destruct ab; reflexivity.
-Qed.
-
-Lemma zeta_inside_ret {A B C}
-  : forall (ab : A * B) (k : A -> B -> C),
-    refine (let (a, b) := ab in ret (k a b))
-           (ret (let (a, b) := ab in k a b)).
-Proof.
-  destruct ab; reflexivity.
-Qed.
-
 Arguments split1' : simpl never.
 Arguments split2' : simpl never.
 Arguments weq : simpl never.
 Arguments natToWord : simpl never.
 Arguments Guarded_Vector_split : simpl never.
+Arguments Core.append_word : simpl never.
 
 Definition refine_simple_encode
   : { b : _ & forall (p : simple_record)
@@ -60,42 +45,37 @@ Definition refine_simple_encode
 Proof.
   unfold Simple_Format_Spec.
   eexists; intros.
-    eapply AlignedEncodeChar; eauto.
-    eapply AlignedEncode2Char; eauto.
-    etransitivity.
-    apply refine_under_bind_both.
-    eapply optimize_align_encode_list.
-    etransitivity.
-    eapply aligned_encode_char_eq.
-    instantiate (1 := fun a ce => (existT _ _ _, _)); simpl.
-    reflexivity.
-    intros; unfold Bind2; simplify with monad laws; higher_order_reflexivity.
-    simpl.
-    match goal with
-      |- context [let (v, c) := ?z in ret (@?b v c)] =>
-      rewrite (zeta_inside_ret z b)
-    end.
-    simplify with monad laws; simpl.
-    rewrite zeta_to_fst; simpl.
-    replace ByteString_id
-      with (build_aligned_ByteString (Vector.nil _)).
-      erewrite <- build_aligned_ByteString_append.
-      reflexivity.
-      eapply ByteString_f_equal;
-        instantiate (1 := eq_refl _); reflexivity.
+  eapply AlignedEncodeChar; eauto.
+  eapply AlignedEncode2Char; eauto.
+  etransitivity.
+  apply refine_under_bind_both.
+  eapply optimize_align_encode_list.
+  etransitivity.
+  eapply aligned_encode_char_eq.
+  instantiate (1 := fun a ce => (existT _ _ _, _)); simpl.
+  reflexivity.
+  intros; unfold Bind2; simplify with monad laws; higher_order_reflexivity.
+  simpl.
+  match goal with
+    |- context [let (v, c) := ?z in ret (@?b v c)] =>
+    rewrite (zeta_inside_ret z _)
+  end.
+  simplify with monad laws; simpl.
+  rewrite zeta_to_fst; simpl.
+  replace ByteString_id
+  with (build_aligned_ByteString (Vector.nil _)).
+  erewrite <- build_aligned_ByteString_append.
+  reflexivity.
+  eapply ByteString_f_equal;
+    instantiate (1 := eq_refl _); reflexivity.
 Defined.
 
 Definition byte_aligned_simple_encoder
              (r : simple_record)
   := Eval simpl in (projT1 refine_simple_encode r).
 
+Import Vectors.VectorDef.VectorNotations.
 Print byte_aligned_simple_encoder.
-
-Ltac rewrite_DecodeOpt2_fmap :=
-  set_refine_evar;
-  progress rewrite ?BindOpt_map, ?DecodeOpt2_fmap_if,
-    ?DecodeOpt2_fmap_if_bool;
-  subst_refine_evar.
 
 Definition Simple_Format_decoder
   : CorrectDecoderFor Simply_OK Simple_Format_Spec.
@@ -111,59 +91,11 @@ Defined.
 Definition SimpleDecoderImpl
     := Eval simpl in (projT1 Simple_Format_decoder).
 
-Lemma Ifopt_Ifopt {A A' B}
-  : forall (a_opt : option A)
-           (t : A -> option A')
-           (e : option A')
-           (t' : A' -> B)
-           (e' :  B),
-    Ifopt (Ifopt a_opt as a Then t a Else e) as a' Then t' a' Else e' =
-                                                Ifopt a_opt as a Then (Ifopt (t a) as a' Then t' a' Else e') Else (Ifopt e as a' Then t' a' Else e').
-Proof.
-  destruct a_opt; simpl; reflexivity.
-Qed.
-
-Corollary AlignedDecodeNat {C}
-            {numBytes}
-    : forall (v : Vector.t (word 8) (S numBytes))
-             (t : _ -> C)
-             e
-             cd,
-    Ifopt (decode_nat (transformerUnit := ByteString_QueueTransformerOpt) 8 (build_aligned_ByteString v) cd) as w
-    Then t w Else e
-     =
-      Let n := wordToNat (Vector.nth v Fin.F1) in
-        t (n, build_aligned_ByteString (snd (Vector_split 1 _ v)), addD cd 8).
-  Proof.
-    unfold CacheDecode.
-    unfold decode_nat, DecodeBindOpt2; intros.
-    unfold BindOpt at 1.
-    rewrite AlignedDecodeChar.
-    reflexivity.
-  Qed.
-
-  Lemma optimize_Guarded_Decode {sz} {C} n
-    : forall (a_opt : ByteString -> C)
-             (a_opt' : ByteString -> C) v c,
-      (~ (n <= sz)%nat
-       -> a_opt (build_aligned_ByteString v) = c)
-      -> (le n sz -> a_opt  (build_aligned_ByteString (Guarded_Vector_split n sz v))
-                     = a_opt'
-                         (build_aligned_ByteString (Guarded_Vector_split n sz v)))
-      -> a_opt (build_aligned_ByteString v) =
-         If NPeano.leb n sz Then
-            a_opt' (build_aligned_ByteString (Guarded_Vector_split n sz v))
-            Else c.
-  Proof.
-    intros; destruct (NPeano.leb n sz) eqn: ?.
-    - apply NPeano.leb_le in Heqb.
-      rewrite <- H0.
-      simpl; rewrite <- build_aligned_ByteString_eq_split'; eauto.
-      eauto.
-    - rewrite H; simpl; eauto.
-      intro.
-      rewrite <- NPeano.leb_le in H1; congruence.
-  Qed.
+  Ltac rewrite_DecodeOpt2_fmap :=
+    set_refine_evar;
+    progress rewrite ?BindOpt_map, ?DecodeOpt2_fmap_if,
+    ?DecodeOpt2_fmap_if_bool;
+    subst_refine_evar.
 
 Definition ByteAligned_SimpleDecoderImpl {A}
            (f : _ -> A)
@@ -176,8 +108,7 @@ Proof.
   etransitivity.
   set_refine_evar; simpl.
   unfold DecodeBindOpt2 at 1; rewrite_DecodeOpt2_fmap.
-  pose CacheEncode.
-  rewrite (@AlignedDecodeNat).
+  rewrite (@AlignedDecodeNat NoCache.test_cache).
   subst_refine_evar; apply rewrite_under_LetIn; intros; set_refine_evar.
   unfold DecodeBindOpt2 at 1; rewrite_DecodeOpt2_fmap.
   rewrite (@AlignedDecode2Char NoCache.test_cache).
@@ -189,7 +120,7 @@ Proof.
   eapply optimize_under_if_opt; simpl; intros.
   higher_order_reflexivity.
   reflexivity.
-  subst_refine_evar; higher_order_reflexivity.
+  Focus 2.
   clear H; intros.
   etransitivity.
   match goal with
@@ -199,16 +130,16 @@ Proof.
       eapply (@optimize_Guarded_Decode n0 _ 1 b')
   end.
   destruct n0 as [ | [ | ?] ]; intros; try omega.
-  pose proof (@decode_word_aligned_ByteString_overflow _ _ 1) as H';
-        simpl in H'; rewrite H'; try reflexivity; auto.
+  apply (@decode_word_aligned_ByteString_overflow NoCache.test_cache) with (sz := 1); auto.
   destruct n0 as [ | ?]; intros; try omega.
   higher_order_reflexivity.
-  instantiate (1 := fun n1 v1 cd0 =>
-                      If NPeano.leb 1 n1 Then (Some ((Vector.hd (Guarded_Vector_split 1 n1 v1), existT _ _ (Vector.tl (Guarded_Vector_split 1 n1 v1))), cd0)) Else None).
+  instantiate (1 := fun n1 v1 (cd0 : CacheDecode) =>
+                      If NPeano.leb 1 n1 Then (Some ((Vector.hd (Guarded_Vector_split 1 n1 v1), @existT _ (Vector.t _) _ (Vector.tl (Guarded_Vector_split 1 n1 v1))), cd0)) Else None).
   simpl; find_if_inside; simpl; try reflexivity.
   pattern n0, v0; apply Vector.caseS; simpl; intros.
   unfold decode_word, WordOpt.decode_word.
   rewrite aligned_decode_char_eq; reflexivity.
+  subst_refine_evar; higher_order_reflexivity.
   higher_order_reflexivity.
 Defined.
 
